Add more pretty instances for error messages.

src/go_lang/interpreter/interpreter.v
@@ -18,6 +18,46 @@ Instance pretty_u64 : Pretty Integers.u64 :=
 Instance pretty_loc : Pretty loc :=
   fun x => pretty x.(loc_car).
 
+Instance pretty_lit : Pretty base_lit :=
+  fun x => match x with
+        | LitInt n => "LitInt"
+        | LitInt32 n => "LitInt32"
+        | LitBool b => "LitBool"
+        | LitByte b => "LitByte"
+        | LitString s => "LitString"
+        | LitUnit => "LitUnit"
+        | LitPoison => "LitPoison"
+        | LitLoc l => "LitLoc"
+        | LitProphecy p => "LitProphecy"
+        end.
+
+Instance pretty_un_op : Pretty un_op := 
+  fun x => match x with
+  | NegOp => "NegOp"
+  | MinusUnOp => "MinusUnOp"
+  | ToUInt64Op => "ToUInt64Op"
+  | ToUInt32Op => "ToUInt32Op"
+  | ToUInt8Op => "ToUInt8Op"
+  end.
+
+Instance pretty_bin_op : Pretty bin_op :=
+  fun x => match x with
+        | PlusOp => "PlusOp"
+        | MinusOp => "MinusOp"
+        | MultOp => "MultOp"
+        | QuotOp => "QuotOp"
+        | RemOp => "RemOp"
+        | AndOp => "AndOp"
+        | OrOp => "OrOp"
+        | XorOp => "XorOp"
+        | ShiftLOp => "ShiftLOp"
+        | ShiftROp => "ShiftROp"
+        | LeOp => "LeOp"
+        | LtOp => "LtOp"
+        | EqOp => "EqOp"
+        | OffsetOp => "OffsetOp"
+        end.
+
 (* The step relation is transitive. Doing n steps and then m steps is
 the same as doing (n + m) steps. Useful in interpret_ok for splitting
 goals like [If e0 e1 e2] ~~> [v] into [If e0 e1 e2] ~~> [If #true e1
@@ -235,6 +275,17 @@ Section interpreter.
   Instance statet_error_ret : MRet (StateT state Error) :=
     StateT_ret Error Error_ret.
 
+  Fixpoint print_val (v: val) : string :=
+    match v with
+    | LitV l => "LitV(" +:+ pretty_lit l +:+ ")"
+    | RecV f x e => "RecV"
+    | PairV v1 v2 => "PairV(" +:+ print_val v1 +:+ ", " +:+ print_val v2 +:+ ")"
+    | InjLV v => "InjL(" +:+ print_val v +:+ ")"
+    | InjRV v => "InjR(" +:+ print_val v +:+ ")"
+    | ExtV x => "ExtV"
+    end.
+  Instance pretty_val : Pretty val := print_val.
+
    (* Given a location l, reads n places from the heap starting at l
    and returns a vec.
    
@@ -369,11 +420,11 @@ Section interpreter.
   (* Interpreter *)
   Fixpoint interpret (fuel: nat) (e: expr) : StateT state Error val :=
     match fuel with
-    | O => mfail "Interpret failed: Fuel depleted"
+    | O => mfail "Fuel depleted"
     | S n =>
       match e with
       | Val v => mret v
-      | Var y => mfail ("Interpret failed: unbound variable " ++ y)
+      | Var y => mfail ("Unbound variable: " ++ y)
       | Rec f y e => mret (RecV f y e)
 
       | App e1 e2 => 
@@ -383,26 +434,28 @@ Section interpreter.
           | RecV f y ex =>
             let e3 := subst' y v2 (subst' f v1 ex) in
             interpret n e3
-          | _ => mfail "Interpret failed: App applied to a non-function"
+          | _ => mfail ("App applied to a non-function of type: " ++ (pretty v1))
           end
             
       | UnOp op e =>
         v <- interpret n e;
-          (* mlift because up_op_eval returns an optional *)
-          mlift (un_op_eval op v) "Interpret failed: UnOp eval returned None"
+          (* mlift because un_op_eval returns an optional *)
+          mlift (un_op_eval op v)
+                ("UnOp eval on invalid type: " ++ (pretty op) ++ "(" ++ (pretty v) ++ ")")
                 
       | BinOp op e1 e2 =>
         v1 <- interpret n e1;
           v2 <- interpret n e2;
-          (* mlift because up_op_eval returns an optional *)
-          mlift (bin_op_eval op v1 v2) "Interpret failed: BinOp eval returned None"
+          (* mlift because bin_op_eval returns an optional *)
+          mlift (bin_op_eval op v1 v2)
+                ("BinOp eval on invalid type: " ++ (pretty op) ++ "(" ++ (pretty v1) ++ ", " ++ (pretty v2) ++ ")")
                 
       | If e0 e1 e2 =>
         c <- interpret n e0;
           match c with
           | LitV (LitBool true) => interpret n e1
           | LitV (LitBool false) => interpret n e2
-          | _ => mfail "Interpret failed: If applied to non-Bool"
+          | _ => mfail ("If applied to non-Bool of type " ++ (pretty c))
           end
 
       | Pair e1 e2 =>
@@ -414,14 +467,14 @@ Section interpreter.
         v <- interpret n e;
           match v with
           | PairV v1 v2 => mret v1
-          | _ => mfail "Interpret failed: Fst applied to non-PairV"
+          | _ => mfail ("Fst applied to non-PairV of type " ++ (pretty v))
           end
 
       | Snd e =>
         v <- interpret n e;
           match v with
           | PairV v1 v2 => mret v2
-          | _ => mfail "Interpret failed: Snd applied to non-PairV"
+          | _ => mfail ("Snd applied to non-PairV of type:" ++ (pretty v))
           end
             
       | InjL e =>
@@ -439,10 +492,10 @@ Section interpreter.
             interpret n (App e1 (Val v'))
           | InjRV v' =>
             interpret n (App e2 (Val v'))
-          | _ => mfail "Interpret failed: Tried to Case on a non-Inj term"
+          | _ => mfail ("Tried to Case on a non-Inj term of type " ++ (pretty v))
           end
 
-      | Fork e => mfail "Interpret failed: Fork operation not supported"
+      | Fork e => mfail "Fork operation not supported"
 
       | Primitive0 p =>
         match p in (prim_op args0) return StateT state Error val with
@@ -464,30 +517,30 @@ Section interpreter.
             match addrv with
             | LitV (LitLoc l) =>
               s <- mget;
-                nav <- mlift (s.(heap) !! l) ("Interpret failed: Load failed for location " ++ (pretty l));
+                nav <- mlift (s.(heap) !! l) ("Load failed for location " ++ (pretty l));
                 match nav with
                 | Reading v 0 => _ <- mupdate (set heap <[l:=Writing]>);
                                   mret (LitV LitUnit)
-                | _ => mfail ("Interpret failed: Race occurred during write at location " ++ (pretty l))
+                | _ => mfail ("Race occurred during write at location " ++ (pretty l))
                 end
-            | _ => mfail "Interpret failed: Attempted Load with a non-location argument"
+            | _ => mfail ("Attempted Load with a non-location argument of type " ++ (pretty addrv))
             end
         | LoadOp =>
           addrv <- interpret n e;
             match addrv with
             | LitV (LitInt l) =>
-              mfail ("Interpret failed: Attempted load at Int " ++ (pretty l) ++ " instead of a Loc")
+              mfail ("Attempted load at Int " ++ (pretty l) ++ " instead of a Loc")
             | LitV (LitLoc l) =>
               (* Since Load of an address with nothing doesn't step,
                  we can lift from the option monad into the StateT option
                  monad here (we mfail "NotImpl" if v is None). *)
               s <- mget;
-                nav <- mlift (s.(heap) !! l) ("Interpret failed: Load failed at location " ++ (pretty l));
+                nav <- mlift (s.(heap) !! l) ("Load failed at location " ++ (pretty l));
                 match nav with
                 | Reading v 0 => mret v
-                | _ => mfail ("Interpret failed: Race detected while reading at location " ++ (pretty l))
+                | _ => mfail ("Race detected while reading at location " ++ (pretty l))
                 end
-            | _ => mfail "Interpret failed: attempted Load with non-location argument"
+            | _ => mfail ("Attempted Load with non-location argument of type " ++ (pretty addrv))
             end
         | InputOp =>
           v <- interpret n e;
@@ -497,7 +550,7 @@ Section interpreter.
                 let x := σ.(oracle) σ.(trace) selv in
                 _ <- mupdate (set trace (fun tr => [In_ev selv (LitInt x)] ++ tr));
                   mret (LitV (LitInt x))
-            | _ => mfail "Interpret failed: attempted InputOp with non-literal selector"
+            | _ => mfail ("Attempted InputOp with non-literal selector of type " ++ (pretty v))
             end
         | OutputOp =>
           v <- interpret n e;
@@ -505,34 +558,34 @@ Section interpreter.
             | LitV v =>
               _ <- mupdate (set trace (fun tr => [Out_ev v] ++ tr));
                 mret (LitV LitUnit)
-            | _ => mfail "Interpret failed: attempted Output with non-literal value"
+            | _ => mfail ("Attempted Output with non-literal value of type " ++ (pretty v))
             end
         | StartReadOp =>
           addrv <- interpret n e;
             match addrv with
             | LitV (LitLoc l) =>
               s <- mget;
-                nav <- mlift (s.(heap) !! l) ("Interpret failed: StartReadOp failed at location " ++ (pretty l));
+                nav <- mlift (s.(heap) !! l) ("StartReadOp failed at location " ++ (pretty l));
                 match nav with
                 | Reading v n => _ <- mupdate (set heap <[l:=Reading v (S n)]>);
                                   mret v
-                | _ => mfail ("Interpret failed: race detected during StartReadOp at location " ++ (pretty l))
+                | _ => mfail ("Race detected during StartReadOp at location " ++ (pretty l))
                 end
-            | _ => mfail "Interpret failed: StartReadOp called with non-location argument"
+            | _ => mfail ("StartReadOp called with non-location argument of type " ++ (pretty addrv))
             end
         | FinishReadOp =>
           addrv <- interpret n e;
             match addrv with
             | LitV (LitLoc l) =>
               s <- mget;
-                nav <- mlift (s.(heap) !! l) ("Interpret failed: FinishReadOp failed at location " ++ (pretty l));
+                nav <- mlift (s.(heap) !! l) ("FinishReadOp failed at location " ++ (pretty l));
                 match nav with
                 | Reading v (S n) => _ <- mupdate (set heap <[l:=Reading v n]>);
                                       mret (LitV LitUnit)
-                | Reading v 0 => mfail ("Interpret failed: FinishReadOp attempted with no reads occurring at location " ++ (pretty l))
-                | _ => mfail ("Interpret failed: attempted FinishReadOp while writing at location " ++ (pretty l))
+                | Reading v 0 => mfail ("FinishReadOp attempted with no reads occurring at location " ++ (pretty l))
+                | _ => mfail ("Attempted FinishReadOp while writing at location " ++ (pretty l))
                 end
-            | _ => mfail "Interpret failed: attempted FinishReadOp with non-location argument"
+            | _ => mfail ("Attempted FinishReadOp with non-location argument of type " ++ (pretty addrv))
             end
         end
 
@@ -544,7 +597,7 @@ Section interpreter.
             match lenv with
             | LitV (LitInt lenz) => 
               if (Z.leb (int.val lenz) 0) then
-                mfail ("Interpret failed: AllocN called with invalid size " ++ (pretty lenz))
+                mfail ("AllocN called with invalid size " ++ (pretty lenz))
               else
                 (* We must allocate a list of length lenz where every entry
                    is initv. state_init_heap does most of the work. *)
@@ -552,7 +605,7 @@ Section interpreter.
                 let l := find_alloc_location s (int.val lenz) in
                 _ <- mput (state_init_heap l (int.val lenz) initv s);
                   mret (LitV (LitLoc l))
-            | _ => @mfail state _ "Interpret failed: AllocN called with with non-integer argument"
+            | _ => @mfail state _ ("AllocN called with with non-integer argument of type " ++ (pretty lenv))
             end
         | FinishStoreOp =>
           addrv <- interpret n e1;
@@ -560,14 +613,14 @@ Section interpreter.
             match addrv with
             | LitV (LitLoc l) => 
               s <- mget;
-                nav <- mlift (s.(heap) !! l) ("Interpret failed: Load failed at location " ++ (pretty l));
+                nav <- mlift (s.(heap) !! l) ("Load failed at location " ++ (pretty l));
                 match nav with
                 | Writing => 
                   _ <- mput (set heap <[l:=Free val]> s);
                     mret (LitV LitUnit)
-                | _ => mfail ("Interpret failed: FinishStoreOp attempted on non-Writing location " ++ (pretty l))
+                | _ => mfail ("FinishStoreOp attempted on non-Writing location " ++ (pretty l))
                 end
-            | _ => @mfail state _ "Interpret failed: attempted Store with non-location argument"
+            | _ => @mfail state _ ("Attempted Store with non-location argument of type " ++ (pretty addrv))
             end
         end
 
@@ -583,19 +636,20 @@ Section interpreter.
             match addrv with
             | LitV (LitLoc l) =>
               s <- mget;
-                nav <- mlift (s.(heap) !! l) ("Interpret failed: CmpXchg load failed at location " ++ (pretty l));
+                nav <- mlift (s.(heap) !! l) ("CmpXchg load failed at location " ++ (pretty l));
                 match nav with
                 | Reading vl 0 =>
-                  b <- mlift (bin_op_eval EqOp vl v1) "Interpret failed: CmpXchg BinOp returned None";
+                  b <- mlift (bin_op_eval EqOp vl v1)
+                    ("CmpXchg BinOp tried on invalid type: " ++ (pretty EqOp) ++ "(" ++ (pretty vl) ++ ", " ++ (pretty v1) ++ ")");
                   match b with
                   | LitV (LitBool true) => _ <- mput (set heap <[l:=Free v2]> s);
                            mret (PairV vl #true)
                   | LitV (LitBool false) => mret (PairV vl #false)
-                  | _ => mfail "Interpret failed: CmpXchg EqOp did not return a boolean"
+                  | _ => mfail ("Expected bool but CmpXchg EqOp returned type: " ++ (pretty b))
                   end
-                | _ => mfail ("Interpret failed: Race detected while reading CmpXchg location " ++ (pretty l))
+                | _ => mfail ("Race detected while reading CmpXchg location " ++ (pretty l))
                 end
-            | _ => mfail "Interpret failed: CmpXchg attempted with non-location argument"
+            | _ => mfail ("CmpXchg attempted with non-location argument of type " ++ (pretty addrv))
             end
 
       (* Won't interpret anything involving prophecy variables. *)
